Almost have a full web server; just needs to parse out 'GET' and 'HTTP/1.1' tokens

platform/tests/WebServerDriver.v
@@ -1,15 +1,36 @@
 Require Import Thread0 WebServer Bootstrap.
 
 
+Module Type HIDE.
+  Parameter heapSize4 : N -> N.
+  Axiom heapSize4_eq : forall n, heapSize4 n = (n * 4)%N.
+
+  Parameter to_nat : N -> nat.
+  Axiom to_nat_eq : to_nat = N.to_nat.
+End HIDE.
+
+Module Hide : HIDE.
+  Definition heapSize4 n := (n * 4)%N.
+  Theorem heapSize4_eq : forall n, heapSize4 n = (n * 4)%N.
+    auto.
+  Qed.
+
+  Definition to_nat := N.to_nat.
+  Theorem to_nat_eq : to_nat = N.to_nat.
+    auto.
+  Qed.
+End Hide.
+
+
 Module Type S.
-  Variable heapSize : nat.
+  Variable heapSize : N.
 End S.
 
 Module Make(M : S).
 Import M.
 
 Module M'.
-  Definition globalSched : W := (heapSize + 50) * 4.
+  Definition globalSched : W := ((heapSize + 50) * 4)%N.
   Definition globalSock : W := globalSched ^+ $4.
   Definition globalTree : W := globalSched ^+ $8.
   Definition globalPages : W := globalSched ^+ $12.
@@ -34,28 +55,60 @@ Module E := WebServer.Make(M').
 Import E.
 
 Section boot.
-  Hypothesis heapSizeLowerBound : (3 <= heapSize)%nat.
+  Definition heapSize' := Hide.to_nat heapSize.
 
-  Definition size := heapSize + 50 + 3.
+  Hypothesis heapSizeLowerBound : (3 <= heapSize)%N.
+
+  Let heapSizeLowerBound' : (3 <= heapSize')%nat.
+    intros; unfold heapSize'; rewrite Hide.to_nat_eq.
+    assert (heapSize >= 3)%N by (apply N.le_ge; auto); nomega.
+  Qed.
+
+  Definition size := heapSize' + 50 + 3.
 
   Hypothesis mem_size : goodSize (size * 4)%nat.
 
-  Let heapSizeUpperBound : goodSize (heapSize * 4).
+  Let heapSizeUpperBound : goodSize (heapSize' * 4).
     goodSize.
   Qed.
+
+  Lemma heapSizeLowerBound'' : natToW 3 <= NToW heapSize.
+    hnf; intros.
+    red in H.
+    pre_nomega.
+    rewrite wordToNat_natToWord_idempotent in H by reflexivity.
+    unfold heapSize' in *.
+    rewrite Hide.to_nat_eq in *.
+    unfold NToW in *.
+    rewrite NToWord_nat in *.
+    rewrite wordToNat_natToWord_idempotent in H.
+    omega.
+    rewrite N2Nat.id.
+    eapply goodSize_weaken in mem_size.
+    2: instantiate (1 := N.to_nat heapSize); unfold size.
+    Transparent goodSize.
+    unfold goodSize in *.
+    rewrite N2Nat.id in *.
+    assumption.
+    unfold heapSize'.
+    rewrite Hide.to_nat_eq.
+    omega.
+  Qed.
+
+  Hint Immediate heapSizeLowerBound''.
 
   Definition bootS := {|
     Reserved := 49;
     Formals := nil;
-    Precondition := fun _ => st ~> Ex n, ![ 0 =?> (heapSize + 50 + 3) * strings n globalPages ] st
+    Precondition := fun _ => st ~> Ex n, ![ 0 =?> (heapSize' + 50 + 3) * strings n globalPages ] st
   |}.
 
   Definition boot := bimport [[ "malloc"!"init" @ [Malloc.initS], "web"!"main" @ [E.mainS] ]]
     bmodule "main" {{
       bfunctionNoRet "main"() [bootS]
-        Sp <- (heapSize * 4)%nat;;
+        Sp <- (heapSize * 4)%N;;
 
-        Assert [Al n, PREmain[_] 0 =?> heapSize * globalSched =?> 3 * strings n globalPages ];;
+        Assert [Al n, PREmain[_] 0 =?> heapSize' * globalSched =?> 3 * strings n globalPages ];;
 
         Call "malloc"!"init"(0, heapSize)
         [Al n, PREmain[_] globalSched =?> 1 * globalSock =?> 1 * globalTree =?> 1 * strings n globalPages
@@ -65,12 +118,69 @@ Section boot.
       end
     }}.
 
-  Ltac t := unfold globalSched, localsInvariantMain, M'.globalSock, M'.globalSched, M'.globalTree, M'.globalPages;
+  Lemma bootstrap_Sp_nonzero : forall sp : W,
+    sp = 0
+    -> sp = (heapSize' * 4)%nat
+    -> goodSize (heapSize' * 4)
+    -> False.
+    intros; eapply bootstrap_Sp_nonzero; try eassumption; eauto.
+  Qed.
+
+  Lemma bootstrap_Sp_freeable : forall sp : W,
+    sp = (heapSize' * 4)%nat
+    -> freeable sp 50.
+    intros; eapply bootstrap_Sp_freeable; try eassumption; eauto.
+  Qed.
+
+  Lemma noWrap : noWrapAround 4 (wordToNat (NToW heapSize) - 1).
+    intros.
+    unfold NToW; rewrite NToWord_nat by auto.
+    unfold heapSize' in *; rewrite Hide.to_nat_eq in *.
+    rewrite wordToNat_natToWord_idempotent.
+    apply noWrap; eauto.
+    eapply goodSize_weaken.
+    2: instantiate (1 := (heapSize' * 4)%nat).
+    unfold heapSize'; rewrite Hide.to_nat_eq; auto.
+    unfold heapSize'; rewrite Hide.to_nat_eq; auto.
+  Qed.
+
+  Local Hint Immediate bootstrap_Sp_nonzero bootstrap_Sp_freeable noWrap.
+
+  Lemma break : NToW ((heapSize + 50) * 4)%N = ((heapSize' + 50) * 4)%nat.
+    intros.
+    unfold NToW; rewrite NToWord_nat by auto.
+    unfold heapSize'; rewrite N2Nat.inj_mul; auto.
+    rewrite Hide.to_nat_eq; rewrite N2Nat.inj_add; auto.
+  Qed.
+
+  Lemma times4 : (Hide.heapSize4 heapSize : W) = (heapSize' * 4)%nat.
+    rewrite Hide.heapSize4_eq; intros.
+    unfold NToW; rewrite NToWord_nat by auto.
+    unfold heapSize'; rewrite N2Nat.inj_mul; auto.
+    rewrite Hide.to_nat_eq; auto.
+  Qed.
+
+  Lemma wordToNat_heapSize : wordToNat (NToW heapSize) = heapSize'.
+    unfold heapSize'; rewrite Hide.to_nat_eq.
+    unfold NToW.
+    rewrite NToWord_nat.
+    apply wordToNat_natToWord_idempotent.
+    eapply goodSize_weaken.
+    2: instantiate (1 := (heapSize' * 4)%nat).
+    auto.
+    unfold heapSize'; rewrite Hide.to_nat_eq; auto.
+  Qed.
+
+  Hint Rewrite break times4 wordToNat_heapSize : sepFormula.
+
+  Ltac t := unfold globalSched, localsInvariantMain, M'.globalSock, M'.globalTree, M'.globalPages, M'.globalSched;
     genesis; rewrite natToW_plus; reflexivity.
 
   Theorem ok0 : moduleOk boot.
-    vcgen; abstract t.
+    unfold boot; rewrite <- Hide.heapSize4_eq; vcgen; abstract t.
   Qed.
+
+  Global Opaque heapSize'.
 
   Definition m1 := link boot E.T.m.
   Definition m2 := link Buffers.m m1.
