platform/tests/WebServerAMD64.v
@@ -1,0 +1,10 @@
+Require Import Bedrock WebServerDriver AMD64_gas.
+
+Module M.
+  Definition heapSize := (1024 * 1024 * 25)%N.
+End M.
+
+Module E := Make(M).
+
+Set Printing Depth 999999.
+Eval compute in moduleS E.m.
